Phi_Semantics/PhiSem_CF_Return.thy
@@ -1,0 +1,12 @@
+theory PhiSem_CF_Return
+  imports Phi_System.PhiSem_Formalization_Tools
+begin
+
+section \<open>Semantic\<close>
+
+virtual_datatype \<phi>CF_return_abnormal = \<phi>empty_abnormal +
+  ER_ret    :: \<open>VAL list\<close> \<comment> \<open>in unit of bits\<close>
+
+print_locale \<phi>CF_return_abnormal
+
+end
